src/model/util.v
@@ -1,9 +1,14 @@
-Require Import Coq.ZArith.ZArith.
+From Coq Require Import Lists.List.
+From Coq Require Import micromega.Lia.
+From Coq Require Import Sorting.Permutation.
+From Coq Require Import ZArith.ZArith.
 
 From compcert Require Import lib.Integers.
 From compcert Require Import common.Values.
 
-Local Open Scope Z.
+From CertiGraph Require Import lib.List_ext.
+
+Import ListNotations.
 
 
 Definition odd_Z2val (x: Z): val
@@ -19,12 +24,14 @@ Definition Z2val (x: Z): val
     else Vint (Int.repr x).
 
 
+Local Open Scope Z.
 Definition range_signed (z: Z) :=
-  (if Archi.ptr64 then Int64.min_signed else Int.min_signed) <= z <=
-  (if Archi.ptr64 then Int64.max_signed else Int.max_signed).
+    (if Archi.ptr64 then Int64.min_signed else Int.min_signed) <= z <=
+    (if Archi.ptr64 then Int64.max_signed else Int.max_signed).
+Local Close Scope Z.
 
 Lemma signed_range_repable_signed (z: Z):
-    Ptrofs.min_signed <= z <= Ptrofs.max_signed <-> range_signed z.
+    (Ptrofs.min_signed <= z <= Ptrofs.max_signed)%Z <-> range_signed z.
 Proof.
     unfold range_signed.
     replace Ptrofs.max_signed
@@ -36,13 +43,13 @@ Proof.
     reflexivity.
 Qed.
 
-Definition repable64_signed (z: Z) := Int64.min_signed <= z <= Int64.max_signed.
+Definition repable64_signed (z: Z) := (Int64.min_signed <= z <= Int64.max_signed)%Z.
   
 Lemma lt64_repr (i j: Z)
     (Hi: repable64_signed i)
     (Hj: repable64_signed j)
     (Hij: Int64.lt (Int64.repr i) (Int64.repr j) = true):
-    i < j.
+    (i < j)%Z.
 Proof.
     unfold Int64.lt in Hij.
     rewrite Int64.signed_repr in Hij ; try assumption.
@@ -54,10 +61,144 @@ Lemma lt64_repr_false (i j: Z)
     (Hi: repable64_signed i)
     (Hj: repable64_signed j)
     (Hij: Int64.lt (Int64.repr i) (Int64.repr j) = false):
-    i >= j.
+    (i >= j)%Z.
 Proof.
     unfold Int64.lt in Hij.
     rewrite Int64.signed_repr in Hij ; try assumption.
     rewrite Int64.signed_repr in Hij ; try assumption.
     now destruct (Coqlib.zlt i j) as [H|H] eqn:E.
+Qed.
+
+
+Fixpoint nat_seq (s total: nat): list nat
+ := match total with
+    | O => nil
+    | S n => s :: nat_seq (S s) n
+    end.
+
+Lemma nat_seq_length (s n: nat):
+    length (nat_seq s n) = n.
+Proof.
+    revert s.
+    induction n as [|n IHn] ; try easy.
+    intro s. simpl. now f_equal.
+Qed.
+
+Lemma nat_seq_S (i num: nat):
+    nat_seq i (S num) = nat_seq i num ++ [num + i].
+Proof.
+    revert i.
+    induction num as [|num IHnum] ; try easy.
+    intro i. remember (S num) as num' eqn:Enum'. simpl.
+    rewrite (IHnum (S i)). subst. simpl.
+    repeat f_equal.
+    lia.
+Qed.
+
+Lemma nat_seq_In_iff (s n i: nat):
+    In i (nat_seq s n) <-> s <= i < s + n.
+Proof.
+    revert s ; induction n as [|n IHn] ; intro s ; simpl.
+    + lia.
+    + rewrite IHn. lia.
+Qed.
+
+Lemma nat_seq_NoDup (s n: nat):
+    NoDup (nat_seq s n).
+Proof.
+    revert s ; induction n as [| n IHn] ; intro s ; simpl ; constructor.
+    + rewrite nat_seq_In_iff. lia.
+    + apply IHn.
+Qed.
+
+Lemma nat_seq_nth (s num n a: nat) (Hn: n < num):
+    nth n (nat_seq s num) a = s + n.
+Proof.
+    revert s n Hn ; induction num as [|num IHnum] ; intros s n Hn ; try lia.
+    destruct n as [|n] ; simpl ; try lia.
+    specialize (IHnum (S s) n) as IHnum.
+    replace (s + S n) with (S s + n) by lia.
+    rewrite IHnum ; lia.
+Qed.
+
+Lemma nat_seq_app (s n m: nat):
+    nat_seq s (n + m) = nat_seq s n ++ nat_seq (s + n) m.
+Proof.
+  revert s ; induction n as [|n IHn] ; intro s ; simpl.
+  + now replace (s + 0) with s by lia.
+  + f_equal.
+    rewrite IHn.
+    now replace (S s + n) with (s + S n) by lia.
+Qed.
+
+Lemma nat_seq_Permutation_cons (s i n: nat) (Hin: i < n):
+    exists l, Permutation (nat_seq s n) (s + i :: l).
+Proof.
+    induction n as [|n IHn] ; try lia.
+    replace (S n) with (n + 1) by lia.
+    rewrite nat_seq_app ; simpl.
+    destruct (Nat.eq_dec i n) as [H|H].
+    - subst.
+      exists (nat_seq s n). symmetry ; apply Permutation_cons_append.
+    - assert (i < n) as Hl by lia.
+      apply IHn in Hl. destruct Hl as [l Hl].
+      exists (l +:: (s + n)).
+      rewrite app_comm_cons.
+      now apply Permutation_app_tail.
+Qed.
+
+Definition nat_inc_list (n: nat): list nat := nat_seq O n.
+
+Lemma nat_inc_list_length (num: nat):
+    length (nat_inc_list num) = num.
+Proof.
+    unfold nat_inc_list.
+    now rewrite nat_seq_length.
+Qed.
+
+Lemma nat_inc_list_S (num: nat):
+    nat_inc_list (S num) = nat_inc_list num ++ [num].
+Proof.
+    unfold nat_inc_list.
+    rewrite nat_seq_S.
+    repeat f_equal.
+    lia.
+Qed.
+
+Lemma nat_inc_list_In_iff (i n: nat):
+    In i (nat_inc_list n) <-> i < n.
+Proof.
+    unfold nat_inc_list.
+    rewrite nat_seq_In_iff.
+    intuition.
+Qed.
+
+Lemma nat_inc_list_nth (i n a: nat) (Hin: i < n):
+    nth i (nat_inc_list n) a = i.
+Proof.
+    unfold nat_inc_list.
+    rewrite nat_seq_nth ; try assumption.
+    lia.
+Qed.
+
+Lemma nat_inc_list_app (n m: nat):
+    nat_inc_list (n + m) = nat_inc_list n ++ nat_seq n m.
+Proof.
+    unfold nat_inc_list.
+    now rewrite nat_seq_app.
+Qed.
+
+Lemma nat_inc_list_NoDup (n: nat):
+    NoDup (nat_inc_list n).
+Proof.
+    unfold nat_inc_list.
+    apply nat_seq_NoDup.
+Qed.
+
+Lemma nat_inc_list_Permutation_cons (i n: nat) (Hin: i < n):
+    exists l, Permutation (nat_inc_list n) (i :: l).
+Proof.
+  unfold nat_inc_list.
+  replace i with (O + i) by lia.
+  now apply nat_seq_Permutation_cons.
 Qed.
